pick StateM for now

Validator/Regex/EnterMem.lean
@@ -6,16 +6,16 @@ import Validator.Regex.Enter
 namespace Regex
 
 def enterM [DecidableEq σ] [Hashable σ] [Monad m] [MonadState (MemTable (@enter σ)) m]
-  (param: Regex σ): m { symbols // symbols = enter param } :=
-  callM enter param
+  (param: Regex σ): m { res // res = enter param } :=
+  MemTable.call enter param
 
 instance [DecidableEq σ] [Hashable σ] [Monad m] [MonadState (MemTable (@enter σ)) m]:
-  Memoize m (α := Regex σ) (β := fun r => Vector σ (symbols r)) enter where
+  Memoize (α := Regex σ) (β := fun r => Vector σ (symbols r)) enter m where
   call param := enterM param
 
 private theorem enterM_is_correct [DecidableEq σ] [Hashable σ] (param: Regex σ) (table: (MemTable (@enter σ))):
   enter param = (StateM.run (s := table) (enterM param)).1 := by
-  have h := call_is_correct (@enter σ) table param
-  unfold call at h
-  unfold enterM
-  rw [h]
+  generalize (StateM.run (enterM param) table) = x
+  obtain ⟨⟨res, hres⟩, table'⟩ := x
+  simp only
+  rw [hres]
